EventSystems/Refinement/Abstract.lean
@@ -1,0 +1,81 @@
+
+/-
+  Reuse of abstract events
+-/
+
+import EventSystems.Refinement.Basic
+
+open Refinement
+
+/-
+ Q : is there a better way to ease the definition of abstract events ? -/
+structure AbstractREventSpec {ACTX} (AM) [Machine ACTX AM]
+                               {CTX} (M) [Machine CTX M]
+                               [Refinement AM M] (α) (β) where
+
+  event : OrdinaryEvent AM α β
+
+  lift (m: M) (x: α) : AM
+
+  lift_ref (m : M) (x : α):
+    Machine.invariant m → refine (lift m x) m
+
+  refine_uniq (am am' : AM) (m : M):
+    Machine.invariant m
+    → refine am m → refine am' m
+    → am = am'
+
+  unlift (am am' : AM) (m : M) (x : α): M
+
+  step_ref (m : M) (x : α):
+    Machine.invariant m
+    → event.guard (lift m x) x
+    → let (_, am') := event.action (lift m x) x
+      refine am' (unlift (lift m x) am' m x)
+
+  step_safe (m : M) (x : α):
+    Machine.invariant m
+    → event.guard (lift m x) x
+    → let (_, am') := event.action (lift m x) x
+      Machine.invariant am' -- redundant but useful
+      → Machine.invariant (unlift (lift m x) am' m x)
+
+@[simp]
+def newAbstractREvent {ACTX} {AM} [Machine ACTX AM]
+                       {CTX} {M} [Machine CTX M]
+                       [instR:Refinement AM M]
+  (abs : AbstractREventSpec AM M α β) : OrdinaryREvent AM M α β :=
+  { guard := fun (m : M) (x : α) => abs.event.guard (abs.lift m x) x
+    action := fun (m : M) (x : α) => let am := abs.lift m x
+                                     let (y, am') := abs.event.action am x
+                                     (y, abs.unlift am am' m x)
+    po := {
+      safety := fun (m : M) (x : α) => by
+        simp
+        intros Hinv Hgrd
+        have Href := abs.lift_ref m x Hinv
+        have Hainv := Refinement.refine_safe (abs.lift m x) m Hinv Href
+        have Hsafe := abs.event.po.safety (abs.lift m x) x Hainv Hgrd
+        apply abs.step_safe m x Hinv Hgrd Hsafe
+
+      abstract := abs.event.to_Event
+
+      strengthening := fun m x => by simp
+                                     intros Hinv Hgrd am Href
+                                     have Href' := abs.lift_ref m x Hinv
+                                     have Ham: am = abs.lift m x := by
+                                       apply abs.refine_uniq am (abs.lift m x) m <;> assumption
+                                     rw [Ham]
+                                     assumption
+
+      simulation := fun m x => by simp
+                                  intros Hinv Hgrd am Href
+                                  have Href' := abs.lift_ref m x Hinv
+                                  have Ham: am = abs.lift m x := by
+                                    apply abs.refine_uniq am (abs.lift m x) m <;> assumption
+                                  rw [Ham]
+                                  constructor
+                                  · simp
+                                  apply abs.step_ref m x Hinv Hgrd
+    }
+  }
